support for simple subrules and almost complete proofs for SystemF example

LottExamples/SystemF.lean
@@ -11,12 +11,38 @@ nonterminal Type', A, B :=
   | a                   : var
   | A " → " B           : arr
   | "∀ " a ". " A       : forall'
+  | "(" A ")"           : paren (desugar := return A)
   | A "[" a " ↦ " B "]" : subst (elab := return mkAppN (.const `LottExamples.SystemF.Type'.subst []) #[A, a, B])
 
 def Type'.subst (A : Type') (a : TypeVar) (B : Type') : Type' := match A with
-  | .var a' => if a' == a then B else .var a'
+  | .var a' => if a' = a then B else .var a'
   | .arr A' B' => .arr (A'.subst a B) (B'.subst a B)
-  | .forall' a' A' => .forall' a' <| if a' == a then A else A'.subst a B
+  | .forall' a' A' => .forall' a' <| if a' = a then A' else A'.subst a B
+
+theorem Type'.forall_subst_eq_subst_forall (aneb : a ≠ b)
+  : [[LottExamples.SystemF.Type'| ∀ a. (A [b ↦ B])]] =
+    [[LottExamples.SystemF.Type'| (∀ a. A) [b ↦ B] ]] := by rw [Type'.subst, if_neg aneb]
+
+theorem Type'.subst_subst : [[LottExamples.SystemF.Type'| A▁target [a ↦ A] [a ↦ B] ]] =
+    [[LottExamples.SystemF.Type'| A▁target [a ↦ A [a ↦ B] ] ]] := by
+  match A_target with
+  | .var a' =>
+    rw [Type'.subst, Type'.subst]
+    split
+    · case isTrue a'eqa => rfl
+    · case isFalse a'nea => rw [Type'.subst, if_neg a'nea]
+  | .arr A' B' =>
+    rw [Type'.subst, Type'.subst]
+    rw [Type'.subst_subst, Type'.subst_subst]
+    rw [← Type'.subst]
+  | .forall' a' A' =>
+    rw [Type'.subst, Type'.subst, Type'.subst]
+    split
+    · case isTrue a'eqa => rfl
+    · case isFalse a'nea => rw [Type'.subst_subst]
+
+theorem Type'.subst_shadowed_forall (B : Type') : [[LottExamples.SystemF.Type'| ∀ a. A]] =
+    [[LottExamples.SystemF.Type'| (∀ a. A) [a ↦ B] ]] := by rw [Type'.subst, if_pos rfl]
 
 nonterminal Term, E, F :=
   | x                     : var
@@ -29,8 +55,8 @@ nonterminal Term, E, F :=
   | E "[" a " ↦ " A "]"   : typeSubst (elab := return mkAppN (.const `LottExamples.SystemF.Term.tySubst []) #[E, a, A])
 
 def Term.tmSubst (E : Term) (x : TermVar) (F : Term) : Term := match E with
-  | .var x' => if x' == x then F else .var x'
-  | .lam x' A E' => .lam x' A <| if x' == x then E' else E'.tmSubst x F
+  | .var x' => if x' = x then F else .var x'
+  | .lam x' A E' => .lam x' A <| if x' = x then E' else E'.tmSubst x F
   | .app E' F' => .app (E'.tmSubst x F) (F'.tmSubst x F)
   | .typeGen a E' => .typeGen a <| E'.tmSubst x F
   | .typeApp E' A => .typeApp (E'.tmSubst x F) A
@@ -39,13 +65,54 @@ def Term.tySubst (E : Term) (a : TypeVar) (A : Type') : Term := match E with
   | .var x => .var x
   | .lam x A' E => .lam x (A'.subst a A) (E.tySubst a A)
   | .app E' F => .app (E'.tySubst a A) (F.tySubst a A)
-  | .typeGen a' E' => .typeGen a' <| if a' == a then E' else E'.tySubst a A
+  | .typeGen a' E' => .typeGen a' <| if a' = a then E' else E'.tySubst a A
   | .typeApp E' A' => .typeApp (E'.tySubst a A) (A'.subst a A)
 
-nonterminal Environment, G :=
-  | "ε"              : empty
-  | G ", " x " : " A : termVarExt
-  | G ", " a         : typeVarExt
+nonterminal Environment, G, GG, GGG :=
+  | "ε"                 : empty
+  | G ", " x " : " A    : termVarExt
+  | G ", " a            : typeVarExt
+  | G ", " GG           : append (elab := return mkAppN (.const `LottExamples.SystemF.Environment.append []) #[G, GG])
+  | "(" G ")"           : paren (desugar := return G)
+  | G "[" a " ↦ " A "]" : subst (elab := return mkAppN (.const `LottExamples.SystemF.Environment.subst []) #[G, a, A])
+
+def Environment.append (G : Environment) : Environment → Environment
+  | .empty => G
+  | .termVarExt G' x A => G.append G' |>.termVarExt x A
+  | .typeVarExt G' a => G.append G' |>.typeVarExt a
+
+theorem Environment.empty_append (G : Environment) : G = Environment.empty.append G := by
+  induction G with
+  | empty => rfl
+  | termVarExt G x A ih => congr
+  | typeVarExt G a ih => congr
+
+def Environment.subst (G : Environment) (a : TypeVar) (A : Type') : Environment :=
+  go G |>.fst
+where
+  go
+    | Environment.empty => (Environment.empty, false)
+    | .termVarExt G' x A' =>
+      let (G'', found) := go G'
+      if found then
+        (G''.termVarExt x A', true)
+      else
+        (G''.termVarExt x (A'.subst a A), false)
+    | .typeVarExt G' a' =>
+      let (G'', found) := go G'
+      (G''.typeVarExt a', a' = a || found)
+
+theorem Environment.subst_empty : Environment.empty = Environment.empty.subst a A := rfl
+
+theorem Environment.subst_typeVarExt_eq_typeVarExt_subst
+  : [[LottExamples.SystemF.Environment| G [b ↦ B], a]] =
+    [[LottExamples.SystemF.Environment| (G, a) [b ↦ B] ]] := rfl
+
+subrule Value, V of Term := lam, typeGen
+
+judgement_syntax a " ≠ " b : TypeVarNe
+
+def TypeVarNe := Ne (α := TypeVar)
 
 judgement_syntax a " ∈ " G : TypeVarInEnvironment
 
@@ -59,10 +126,156 @@ a ∈ G
 a ∈ G, x : A
 
 a ∈ G
-──────── typeVarExt
-a ∈ G, b
+a ≠ a▁other
+────────────── typeVarExt
+a ∈ G, a▁other
 
-example : ¬[[a ∈ ε]] := by intro h; cases h
+judgement_syntax a " ∉ " G : TypeVarNotInEnvironment
+
+set_option linter.unusedVariables false in
+def TypeVarNotInEnvironment a G := ¬[[a ∈ G]]
+
+theorem TypeVarInEnvironment.append_elim (ainGappGG : [[a ∈ G, GG]]) : [[a ∈ G]] ∨ [[a ∈ GG]] := by
+  by_cases [[a ∈ GG]]
+  · case pos ainGG => exact .inr ainGG
+  · case neg aninGG =>
+    left
+    induction GG
+    · case empty => exact ainGappGG
+    · case termVarExt GG' x A ih =>
+      apply ih
+      · cases ainGappGG
+        case ainGappGG.termVarExt => assumption
+      · intro ainGG'
+        exact aninGG ainGG'.termVarExt
+    · case typeVarExt GG' a' ih =>
+      by_cases a' = a
+      · case pos a'eqa =>
+        apply False.elim
+        apply aninGG
+        rw [a'eqa]
+        exact .head
+      · case neg a'nea =>
+        apply ih
+        · cases ainGappGG
+          · case ainGappGG.head => contradiction
+          · case ainGappGG.typeVarExt => assumption
+        · intro ainGG'
+          apply aninGG
+          have a'nea : a' ≠ a := a'nea
+          exact ainGG'.typeVarExt a'nea.symm
+
+theorem TypeVarInEnvironment.append_inl (ainG : [[a ∈ G]]) : [[a ∈ G, GG]] := by
+  match GG with
+  | .empty => exact ainG
+  | .termVarExt GG' x A => exact ainG.append_inl |>.termVarExt
+  | .typeVarExt GG' a' =>
+    by_cases a' = a
+    · case pos a'eqa =>
+      rw [a'eqa]
+      exact .head
+    · case neg a'nea =>
+      have a'nea : a' ≠ a := a'nea
+      exact .typeVarExt ainG.append_inl a'nea.symm
+
+theorem TypeVarInEnvironment.append_inr : [[a ∈ GG]] → [[a ∈ G, GG]]
+  | .head => .head
+  | .termVarExt ainGG' => ainGG'.append_inr |>.termVarExt
+  | .typeVarExt ainGG' anea' => ainGG'.append_inr |>.typeVarExt anea'
+
+theorem TypeVarInEnvironment.subst (ainG : [[a ∈ G]]) : [[a ∈ G [b ↦ A] ]] := by
+  rw [Environment.subst]
+  induction G
+  · case empty => cases ainG
+  · case termVarExt G' x A' ih =>
+    rw [Environment.subst.go]
+    simp
+    split <;>
+    · simp
+      apply TypeVarInEnvironment.termVarExt
+      apply ih
+      cases ainG
+      case a.termVarExt ainG' =>
+      exact ainG'
+  · case typeVarExt G' a' ih =>
+    rw [Environment.subst.go]
+    simp
+    cases ainG
+    · case head => exact .head
+    · case typeVarExt ainG' anea' =>
+      apply TypeVarInEnvironment.typeVarExt _ anea'
+      apply ih
+      exact ainG'
+
+theorem TypeVarNotInEnvironment.termVarExt (aninG : [[a ∉ G]]) : [[a ∉ G, x : A]] := by
+  intro ainGx
+  apply aninG
+  cases ainGx
+  case termVarExt ainG => exact ainG
+
+theorem TypeVarNotInEnvironment.typeVarExt (aninG : [[a ∉ G]]) (bnea : b ≠ a) : [[a ∉ G, b]] := by
+  intro ainGa
+  apply aninG
+  cases ainGa
+  · case head => contradiction
+  · case typeVarExt ainG _ => exact ainG
+
+theorem TypeVarNotInEnvironment.TermVar_drop (aninGx : [[a ∉ G, x : A]]) : [[a ∉ G]] := by
+  intro ainG
+  exact aninGx ainG.termVarExt
+
+theorem TypeVarNotInEnvironment.TypeVar_drop (aninGb : [[a ∉ G, b]]) : [[a ∉ G]] := by
+  intro ainG
+  by_cases a = b
+  · case pos aeqb =>
+    rw [aeqb] at aninGb
+    exact aninGb .head
+  · case neg aneb => exact aninGb <| ainG.typeVarExt aneb
+
+theorem Environment.subst_go_snd_eq_false_of_TermVarNotInEnvironment G (aninG : [[a ∉ G]])
+  : (Environment.subst.go a A G).snd = false := by
+  cases G
+  · case empty => rfl
+  · case termVarExt G' x A' =>
+    rw [subst.go]
+    split
+    split
+    · case isTrue q r found receq foundeqtrue =>
+      apply ne_false_of_eq_true (b := (subst.go a A G').snd)
+      · simp [foundeqtrue, receq]
+      · apply G'.subst_go_snd_eq_false_of_TermVarNotInEnvironment
+        exact aninG.TermVar_drop
+    · case isFalse => simp
+  · case typeVarExt G' a' =>
+    rw [subst.go]
+    simp
+    have a'nea : a' ≠ a := by
+      intro a'eqa
+      rw [a'eqa] at aninG
+      apply aninG
+      exact .head
+    constructor
+    · exact a'nea
+    · apply G'.subst_go_snd_eq_false_of_TermVarNotInEnvironment
+      exact aninG.TypeVar_drop
+
+theorem Environment.subst_termVarExt_eq_termVarExt_subst_of_TypeVarNotInEnvironment
+  (aninG : [[a ∉ G]]) : [[LottExamples.SystemF.Environment| G [a ↦ B], x : (A [a ↦ B])]] =
+    [[LottExamples.SystemF.Environment| (G, x : A) [a ↦ B] ]] := by
+  rw [Environment.subst, Environment.subst, subst.go]
+  simp
+  split
+  · case isTrue sndeqtrue =>
+    apply False.elim
+    apply ne_false_of_eq_true sndeqtrue
+    exact G.subst_go_snd_eq_false_of_TermVarNotInEnvironment aninG
+  · case isFalse => simp
+
+theorem TypeVarNotInEnvironment.ε : [[a ∉ ε]] := fun ainε => by cases ainε
+
+judgement_syntax x " ≠ " y : TermVarNe
+
+def TermVarNe := Ne (α := TermVar)
 
 judgement_syntax x " : " A " ∈ " G : TermVarInEnvironment
 
@@ -72,61 +285,933 @@ judgement TermVarInEnvironment :=
 x : A ∈ G, x : A
 
 x : A ∈ G
-──────────────── termVarExt
-x : A ∈ G, y : B
+x ≠ x▁other
+────────────────────── termVarExt
+x : A ∈ G, x▁other : B
 
 x : A ∈ G
 ──────────── typeVarExt
 x : A ∈ G, a
 
-example : ¬[[x : A ∈ ε]] := by intro h; cases h
+judgement_syntax x " ∉ " G : TermVarNotInEnvironment
 
-judgement_syntax G " |- " A : TypeWellFormedness
+set_option linter.unusedVariables false in
+def TermVarNotInEnvironment x G := ∀ A : Type', ¬[[x : A ∈ G]]
+
+theorem TermVarInEnvironment.append_elim (xAinGappGG : [[x : A ∈ G, GG]])
+  : [[x : A ∈ G]] ∧ [[x ∉ GG]] ∨ [[x : A ∈ GG]] := by
+  by_cases [[x : A ∈ GG]]
+  · case pos xAinGG => exact .inr xAinGG
+  · case neg xAninGG =>
+    left
+    match GG with
+    | .empty =>
+      constructor
+      · exact xAinGappGG
+      · intro A'
+        intro xA'inε
+        cases xA'inε
+    | .termVarExt GG' x' A' =>
+      by_cases x' = x
+      · case pos x'eqx =>
+        by_cases A' = A
+        · case pos A'eqA =>
+          rw [x'eqx, A'eqA] at xAinGappGG xAninGG
+          exact False.elim <| xAninGG .head
+        · case neg A'neA =>
+          cases xAinGappGG
+          · case head => contradiction
+          · case termVarExt xAinGappGG' xnex' =>
+            exact False.elim <| xnex' x'eqx.symm
+      · case neg x'nex =>
+        cases xAinGappGG
+        · case head => contradiction
+        · case termVarExt xAinGappGG' xnex' =>
+          rcases xAinGappGG'.append_elim with ⟨xAinG, xninGG'⟩ | xAinG''
+          · constructor
+            · exact xAinG
+            · intro A''
+              intro xA''inGG'x'A'
+              match xA''inGG'x'A' with
+              | .head => contradiction
+              | .termVarExt xA''inG'  _ => exact xninGG' A'' xA''inG'
+          · have x'nex : x' ≠ x := x'nex
+            exact False.elim <| xAninGG <| xAinG''.termVarExt x'nex.symm
+    | .typeVarExt GG' a =>
+      cases xAinGappGG
+      case typeVarExt xAinGappG'' =>
+      match xAinGappG''.append_elim with
+      | .inl ⟨xAinG, xninGG'⟩ =>
+        constructor
+        · exact xAinG
+        · intro A' xA'inGG'a
+          apply xninGG' A'
+          cases xA'inGG'a
+          case right.typeVarExt xA'inGG' =>
+          exact xA'inGG'
+      | .inr xAinGG' =>
+        exact False.elim <| xAninGG xAinGG'.typeVarExt
+
+theorem TermVarInEnvironment.append_inl (xAinG : [[x : A ∈ G]]) (xninGG : [[x ∉ GG]])
+  : [[x : A ∈ G, GG]] := by
+  match GG with
+  | .empty => exact xAinG
+  | .termVarExt GG' x' A' =>
+    by_cases x' = x
+    · case pos x'eqx =>
+      rw [x'eqx]
+      rw [x'eqx] at xninGG
+      exact False.elim <| xninGG A' .head
+    · case neg x'nex =>
+      have x'nex : x' ≠ x := x'nex
+      apply TermVarInEnvironment.termVarExt _ x'nex.symm
+      apply xAinG.append_inl
+      intro A'' xA''inGG'
+      apply xninGG A''
+      exact .termVarExt xA''inGG' x'nex.symm
+  | .typeVarExt GG' a =>
+    apply TermVarInEnvironment.typeVarExt
+    apply xAinG.append_inl
+    intro A' xA'inGG'
+    exact xninGG A' xA'inGG'.typeVarExt
+
+theorem TermVarInEnvironment.append_inr : [[x : A ∈ GG]] → [[x : A ∈ G, GG]]
+  | .head => .head
+  | .termVarExt xAinGG' xnex' => xAinGG'.append_inr |>.termVarExt xnex'
+  | .typeVarExt xAinGG' => xAinGG'.append_inr |>.typeVarExt
+
+theorem TermVarInEnvironment.TermVar_swap (xtinGxyGG : [[x▁target : A▁target ∈ G, x : A, y : B, GG]])
+  (xney : x ≠ y) : [[x▁target : A▁target ∈ G, y : B, x : A, GG]] := by
+  match xtinGxyGG.append_elim with
+  | .inl ⟨xtinGxy, xtninGG⟩ =>
+    apply TermVarInEnvironment.append_inl _ xtninGG
+    match xtinGxy with
+    | .head => exact .termVarExt .head xney.symm
+    | .termVarExt xtinGx xtney => match xtinGx with
+      | .head => exact .head
+      | .termVarExt xtinG xtnex => exact xtinG.termVarExt xtney |>.termVarExt xtnex
+  | .inr xtinGG => exact xtinGG.append_inr
+
+theorem TermVarInEnvironment.subst (xAinG : [[x : A ∈ G]]) (aninG : [[a ∉ G]])
+  : [[x : A [a ↦ B] ∈ G [a ↦ B] ]] := by
+  rw [Environment.subst]
+  induction G
+  · case empty => cases xAinG
+  · case termVarExt G' x' A' ih =>
+    rw [Environment.subst.go]
+    simp
+    split
+    · case isTrue sndeqtrue =>
+      apply False.elim
+      apply ne_false_of_eq_true sndeqtrue
+      apply G'.subst_go_snd_eq_false_of_TermVarNotInEnvironment
+      exact aninG.TermVar_drop
+    · case isFalse sndeqfalse =>
+      cases xAinG
+      · case head => exact .head
+      · case termVarExt xAinG' xnex' =>
+        apply TermVarInEnvironment.termVarExt _ xnex'
+        apply ih xAinG'
+        exact aninG.TermVar_drop
+  · case typeVarExt G' a' ih =>
+    rw [Environment.subst.go]
+    simp
+    cases xAinG
+    case typeVarExt xAinG' =>
+    apply TermVarInEnvironment.typeVarExt
+    apply ih xAinG'
+    exact aninG.TypeVar_drop
+
+set_option linter.unusedVariables false in
+theorem TermVarInEnvironment.unsubst (xAsinGs : [[x : A▁target ∈ G [a ↦ B] ]]) (aninG : [[a ∉ G]])
+  : ∃ A, [[x : A ∈ G]] ∧ A_target = [[LottExamples.SystemF.Type'| A [a ↦ B] ]] := by
+  rw [Environment.subst] at xAsinGs
+  induction G
+  · case empty => cases xAsinGs
+  · case termVarExt G' x' A' ih =>
+    rw [Environment.subst.go] at xAsinGs
+    simp at xAsinGs
+    split at xAsinGs
+    · case isTrue sndeqtrue =>
+      apply False.elim
+      apply ne_false_of_eq_true sndeqtrue
+      apply G'.subst_go_snd_eq_false_of_TermVarNotInEnvironment
+      exact aninG.TermVar_drop
+    · case isFalse sndeqfalse =>
+      simp at xAsinGs
+      cases xAsinGs
+      · case head => exact Exists.intro A' ⟨.head, rfl⟩
+      · case termVarExt xAinG' xnex' =>
+        let ⟨A'', ⟨xA''inG', eq⟩⟩ := ih xAinG' aninG.TermVar_drop
+        exact Exists.intro A'' ⟨xA''inG'.termVarExt xnex', eq⟩
+  · case typeVarExt G' a' ih =>
+    rw [Environment.subst.go] at xAsinGs
+    simp at xAsinGs
+    cases xAsinGs
+    case typeVarExt xAinG' =>
+    let ⟨A', ⟨xA'inG', eq⟩⟩ := ih xAinG' aninG.TypeVar_drop
+    exact Exists.intro A' ⟨xA'inG'.typeVarExt, eq⟩
+
+theorem TermVarNotInEnvironment.ε : [[x ∉ ε]] := fun _ xinε => by cases xinε
+
+theorem TermVarNotInEnvironment.termVarExt (xninG : [[x ∉ G]]) (ynex : y ≠ x)
+  : [[x ∉ G, y : A]] := by
+  intro A' xA'inGy
+  apply xninG A'
+  cases xA'inGy
+  · case head => contradiction
+  · case termVarExt xA'inG _ => exact xA'inG
+
+theorem TermVarNotInEnvironment.typeVarExt (xninG : [[x ∉ G]]) : [[x ∉ G, a]] := by
+  intro A' xA'inGa
+  apply xninG A'
+  cases xA'inGa
+  case typeVarExt xA'inG => exact xA'inG
+
+judgement_syntax G " ⊢ " A : TypeWellFormedness
 
 judgement TypeWellFormedness :=
 
 a ∈ G
-────── var
-G |- a
+───── var
+G ⊢ a
 
-G |- A
-G |- B
-────────── arr
-G |- A → B
+G ⊢ A
+G ⊢ B
+───────── arr
+G ⊢ A → B
 
-G, a |- A
-─────────── forall'
-G |- ∀ a. A
+G, a ⊢ A
+────────── forall'
+G ⊢ ∀ a. A
 
-judgement_syntax G " |- " E " : " A : Typing
+theorem TypeWellFormedness.TypeVar_swap (Awf : [[G, b, a, GG ⊢ A]]) : [[G, a, b, GG ⊢ A]] := by
+  cases Awf
+  · case var a' a'inGbaGG =>
+    match a'inGbaGG.append_elim with
+    | .inl a'inGba =>
+      cases a'inGba
+      · case head =>
+        by_cases a = b
+        · case pos aeqb =>
+          rw [aeqb]
+          exact .var TypeVarInEnvironment.head.append_inl
+        · case neg aneb =>
+          exact .var <| .append_inl <| .typeVarExt .head aneb
+      · case typeVarExt a'inGb a'nea =>
+        cases a'inGb
+        · case head => exact .var <| .append_inl .head
+        · case typeVarExt a'inG a'neb =>
+          exact .var <| .append_inl <| .typeVarExt (.typeVarExt a'inG a'nea) a'neb
+    | .inr a'inGG => exact .var a'inGG.append_inr
+  · case arr A' B A'wf Bwf =>
+    exact .arr A'wf.TypeVar_swap Bwf.TypeVar_swap
+  · case forall' a' A' A'wf =>
+    apply TypeWellFormedness.forall'
+    rw [← Environment.append]
+    exact TypeWellFormedness.TypeVar_swap A'wf
+
+theorem TypeWellFormedness.TypeVar_shadowed : [[G, a, a ⊢ A]] → [[G, a ⊢ A]]
+  | .var a'inGaa => match a'inGaa with
+    | .head => .var .head
+    | .typeVarExt a'inGa _ => .var a'inGa
+  | .arr A'wf Bwf => .arr A'wf.TypeVar_shadowed Bwf.TypeVar_shadowed
+  | .forall' A'wf => .forall' <| A'wf.TypeVar_swap (GG := .empty)
+      |>.TypeVar_swap (GG := .typeVarExt .empty a)
+      |>.TypeVar_shadowed
+      |>.TypeVar_swap (GG := .empty)
+
+theorem TypeWellFormedness.TermVar_drop : [[G, x : A, GG ⊢ B]] → [[G, GG ⊢ B]]
+  | .var ainGxGG => match ainGxGG.append_elim with
+    | .inl (.termVarExt ainG) => .var ainG.append_inl
+    | .inr ainGG => .var ainGG.append_inr
+  | .arr A'wf B'wf => .arr A'wf.TermVar_drop B'wf.TermVar_drop
+  | .forall' A'wf => .forall' <| A'wf.TermVar_drop (GG := .typeVarExt GG _)
+
+theorem TypeWellFormedness.TermVar_intro : [[G, GG ⊢ B]] → [[G, x : A, GG ⊢ B]]
+  | .var ainGappGG => match ainGappGG.append_elim with
+    | .inl ainG => .var ainG.termVarExt.append_inl
+    | .inr ainGG => .var ainGG.append_inr
+  | .arr A'wf B'wf => .arr A'wf.TermVar_intro B'wf.TermVar_intro
+  | .forall' A'wf => .forall' <| A'wf.TermVar_intro (GG := .typeVarExt GG _)
+
+theorem TypeWellFormedness.TermVar_swap (Bwf : [[G, y : A▁other, x : A, GG ⊢ B]])
+  : [[G, x : A, y : A▁other, GG ⊢ B]] := Bwf.TermVar_drop.TermVar_drop.TermVar_intro.TermVar_intro
+
+theorem TypeWellFormedness.append_inr : [[G ⊢ A]] → [[GG, G ⊢ A]]
+  | .var ainG => .var ainG.append_inr
+  | .arr A'wf Bwf => .arr A'wf.append_inr Bwf.append_inr
+  | .forall' A'wf => .forall' A'wf.append_inr
+
+theorem TypeWellFormedness.TypeVar_shadowed_subst
+  : [[ε, a, G, a, GG ⊢ A]] → [[(G, a) [a ↦ B], GG ⊢ A]]
+  | .var a'inεaGaGG =>
+    match a'inεaGaGG.append_elim with
+    | .inl a'inεa =>
+      match a'inεa with
+      | .head => .var TypeVarInEnvironment.head.subst.append_inl
+      | .typeVarExt a'inε _ => by cases a'inε
+    | .inr a'inGaGG => match a'inGaGG.append_elim with
+      | .inl a'inGa => .var a'inGa.subst.append_inl
+      | .inr a'inGG => .var a'inGG.append_inr
+  | .arr A'wf B'wf => .arr A'wf.TypeVar_shadowed_subst B'wf.TypeVar_shadowed_subst
+  | .forall' A'wf => .forall' <| A'wf.TypeVar_shadowed_subst (GG := GG.typeVarExt _)
+
+theorem TypeWellFormedness.subst (Awf : [[ε, a, G ⊢ A]]) (Bwf : [[ε ⊢ B]])
+  : [[G [a ↦ B] ⊢ A [a ↦ B] ]] := by
+  cases Awf
+  · case var a' a'inεaG =>
+    rw [Type'.subst]
+    split
+    · case isTrue a'eqa =>
+      exact Bwf.append_inr
+    · case isFalse a'nea =>
+      match a'inεaG.append_elim with
+      | .inl a'inεa =>
+        cases a'inεa
+        · case head => contradiction
+        · case typeVarExt => contradiction
+      | .inr a'inG =>
+        exact .var a'inG.subst
+  · case arr A' B' A'wf B'wf => exact .arr (A'wf.subst Bwf) (B'wf.subst Bwf)
+  · case forall' a' A' A'wf =>
+    rw [Type'.subst]
+    split
+    · case isTrue a'eqa =>
+      rw [a'eqa]
+      rw [a'eqa] at A'wf
+      exact .forall' <| A'wf.TypeVar_shadowed_subst (GG := .empty)
+    · case isFalse a'nea => exact TypeWellFormedness.forall' <| A'wf.subst (G := G.typeVarExt a') Bwf
+
+theorem Type'.subst_id_of_TypeWellFormedness_of_TypeVarNotInEnvironment (Awf : [[G ⊢ A]])
+  (aninG : [[a ∉ G]]) : [[LottExamples.SystemF.Type'| A [a ↦ B] ]] = A := by
+  match Awf with
+  | .var a'inG =>
+    rw [Type'.subst]
+    split
+    · case isTrue a'eqa =>
+      rw [a'eqa] at a'inG
+      exact False.elim <| aninG a'inG
+    · case isFalse => rfl
+  | .arr A'wf B'wf =>
+    rw [Type'.subst, Type'.subst_id_of_TypeWellFormedness_of_TypeVarNotInEnvironment A'wf aninG,
+        Type'.subst_id_of_TypeWellFormedness_of_TypeVarNotInEnvironment B'wf aninG]
+  | .forall' A'wf =>
+    rw [Type'.subst]
+    split
+    · case isTrue => rfl
+    · case isFalse a'nea =>
+      rw [Type'.subst_id_of_TypeWellFormedness_of_TypeVarNotInEnvironment A'wf]
+      exact aninG.typeVarExt a'nea
+
+judgement_syntax a " ∈ " "ftv" "(" A ")" : InFreeTypeVars
+
+judgement InFreeTypeVars :=
+
+────────── var
+a ∈ ftv(a)
+
+a ∈ ftv(A)
+────────────── arrl
+a ∈ ftv(A → B)
+
+a ∈ ftv(B)
+────────────── arrr
+a ∈ ftv(A → B)
+
+a ∈ ftv(A)
+a ≠ b
+─────────────── forall'
+a ∈ ftv(∀ b. A)
+
+judgement_syntax a " ∉ " "ftv" "(" A ")" : NotInFreeTypeVars
+
+set_option linter.unusedVariables false in
+def NotInFreeTypeVars a A := ¬[[a ∈ ftv(A)]]
+
+theorem NotInFreeTypeVars.of_TypeWellFormedness_of_TypeVarNotInEnvironment (Awf : [[G ⊢ A]])
+  (aninG : [[a ∉ G]]) : [[a ∉ ftv(A)]] := by
+  intro ain
+  match A, Awf with
+  | .var a', .var a'inG =>
+    let .var := ain
+    exact aninG a'inG
+  | .arr A' B, .arr A'wf Bwf => match ain with
+    | .arrl ainA' =>
+      exact NotInFreeTypeVars.of_TypeWellFormedness_of_TypeVarNotInEnvironment A'wf aninG <| ainA'
+    | .arrr ainB =>
+      exact NotInFreeTypeVars.of_TypeWellFormedness_of_TypeVarNotInEnvironment Bwf aninG <| ainB
+  | .forall' a' A', .forall' A'wf =>
+    let .forall' ainftvA' anea' := ain
+    apply NotInFreeTypeVars.of_TypeWellFormedness_of_TypeVarNotInEnvironment A'wf _ ainftvA'
+    exact aninG.typeVarExt anea'.symm
+
+theorem InFreeTypeVars.unsubst (ain : [[a ∈ ftv(A [b ↦ B])]]) (Bwf : [[ε ⊢ B]]) : [[a ∈ ftv(A)]] := by
+  match A with
+  | .var a' =>
+    rw [Type'.subst] at ain
+    split at ain
+    · case isTrue a'eqa =>
+      exact False.elim <|
+        NotInFreeTypeVars.of_TypeWellFormedness_of_TypeVarNotInEnvironment Bwf
+          TypeVarNotInEnvironment.ε ain
+    · case isFalse a'neb =>
+      let .var := ain
+      exact .var
+  | .arr A' B' =>
+    rw [Type'.subst] at ain
+    match ain with
+    | .arrl ain => exact .arrl <| ain.unsubst Bwf
+    | .arrr ain => exact .arrr <| ain.unsubst Bwf
+  | .forall' a' A' =>
+    rw [Type'.subst] at ain
+    split at ain
+    · case isTrue a'eqb => exact ain
+    · case isFalse a'neb =>
+      let .forall' ain anea' := ain
+      exact .forall' (ain.unsubst Bwf) anea'
+
+theorem NotInFreeTypeVars.subst_id (aninftvA : [[a ∉ ftv(A)]])
+  : [[LottExamples.SystemF.Type'| A [a ↦ B] ]] = A := by
+  match A with
+  | .var a' =>
+    rw [Type'.subst, if_neg]
+    intro a'eqa
+    rw [a'eqa] at aninftvA
+    exact aninftvA .var
+  | .arr A' B' =>
+    rw [Type'.subst, NotInFreeTypeVars.subst_id, NotInFreeTypeVars.subst_id]
+    · intro ainftvB'
+      exact aninftvA <| .arrr ainftvB'
+    · intro ainftvA'
+      exact aninftvA <| .arrl ainftvA'
+  | .forall' a' A' =>
+    rw [Type'.subst]
+    split
+    · case isTrue => rfl
+    · case isFalse a'nea =>
+      have a'nea : a' ≠ a := a'nea
+      rw [NotInFreeTypeVars.subst_id]
+      intro ainftvA'
+      exact aninftvA <| InFreeTypeVars.forall' ainftvA' a'nea.symm
+
+judgement_syntax x " ∈ " "fv" "(" E ")" : InFreeTermVars
+
+judgement InFreeTermVars :=
+
+───────── var
+x ∈ fv(x)
+
+x ∈ fv(E)
+x ≠ y
+────────────────── lam
+x ∈ fv(λ y : A. E)
+
+x ∈ fv(E)
+─────────── appl
+x ∈ fv(E F)
+
+x ∈ fv(F)
+─────────── appr
+x ∈ fv(E F)
+
+x ∈ fv(E)
+───────────── typeGen
+x ∈ fv(Λ a. E)
+
+x ∈ fv(E)
+───────────── typeApp
+x ∈ fv(E [A])
+
+judgement_syntax x " ∉ " "fv" "(" E ")" : NotInFreeTermVars
+
+set_option linter.unusedVariables false in
+def NotInFreeTermVars x E := ¬[[x ∈ fv(E)]]
+
+judgement_syntax G " ⊢ " a " ∈ " "fvftv" "(" E ")" : InFreeTermVars'Types'FreeTypeVars
+
+judgement InFreeTermVars'Types'FreeTypeVars :=
+
+x ∈ fv(E)
+x : A ∈ G
+a ∈ ftv(A)
+───────── mk
+G ⊢ a ∈ fvftv(E)
+
+judgement_syntax G " ⊢ " a " ∉ " "fvftv" "(" E ")" : NotInFreeTermVars'Types'FreeTypeVars
+
+set_option linter.unusedVariables false in
+def NotInFreeTermVars'Types'FreeTypeVars G a E := ¬[[G ⊢ a ∈ fvftv(E)]]
+
+theorem NotInFreeTermVars'Types'FreeTypeVars.TermVar_swap
+  (anin : [[G, y : A▁other, x : A, GG ⊢ a ∉ fvftv(E)]]) (xney : x ≠ y)
+  : [[G, x : A, y : A▁other, GG ⊢ a ∉ fvftv(E)]] := by
+  intro ain
+  apply anin
+  let .mk x'infv x'A'in ainftvA' := ain
+  exact InFreeTermVars'Types'FreeTypeVars.mk x'infv (x'A'in.TermVar_swap xney) ainftvA'
+
+theorem NotInFreeTermVars'Types'FreeTypeVars.TermVar_shadowed (anin : [[G, x : A▁shadowed, GG, x : A, GGG ⊢ a ∉ fvftv(E)]])
+  : [[G, GG, x : A, GGG ⊢ a ∉ fvftv(E)]] := by
+  intro ain
+  apply anin
+  cases ain
+  case mk x' A' x'A'in ainftvA' x'infv =>
+  apply InFreeTermVars'Types'FreeTypeVars.mk x'infv _ ainftvA'
+  match x'A'in.append_elim with
+  | .inl ⟨x'A'inG, x'ninGGxGGG⟩ =>
+    apply TermVarInEnvironment.append_inl _ x'ninGGxGGG
+    by_cases x' = x
+    · case pos x'eqx =>
+      apply False.elim
+      rw [x'eqx] at x'ninGGxGGG
+      apply x'ninGGxGGG A
+      apply TermVarInEnvironment.head.append_inl
+      intro A'' xA''inGG
+      apply x'ninGGxGGG A''
+      exact xA''inGG.append_inr
+    · case neg x'nex => exact x'A'inG.termVarExt x'nex
+  | .inr x'A'inGGxGGG => exact x'A'inGGxGGG.append_inr
+
+theorem NotInFreeTermVars'Types'FreeTypeVars.append_elr (anin : [[G, GG ⊢ a ∉ fvftv(E)]])
+  : [[GG ⊢ a ∉ fvftv(E)]] := by
+  intro ain
+  apply anin
+  let .mk x'infv x'A'inG ainftv := ain
+  exact InFreeTermVars'Types'FreeTypeVars.mk x'infv x'A'inG.append_inr ainftv
+
+theorem NotInFreeTermVars'Types'FreeTypeVars.Environment_subst (anin : [[G ⊢ a ∉ fvftv(E)]])
+  (Awf : [[ε ⊢ A]]) (bninG : [[b ∉ G]]) : [[G [b ↦ A] ⊢ a ∉ fvftv(E)]] := by
+  intro ain
+  apply anin
+  let .mk x'infv x'A'inG ainftv := ain
+  let ⟨_, ⟨xA'inG', eq⟩⟩ := x'A'inG.unsubst bninG
+  rw [eq] at ainftv
+  exact .mk x'infv xA'inG' <| ainftv.unsubst Awf
+
+theorem NotInFreeTermVars'Types'FreeTypeVars.appl (anin : [[G ⊢ a ∉ fvftv(E F)]])
+  : [[G ⊢ a ∉ fvftv(E)]] := by
+  intro ain
+  apply anin
+  let .mk x'infv x'A'inG ainftv := ain
+  exact .mk x'infv.appl x'A'inG ainftv
+
+theorem NotInFreeTermVars'Types'FreeTypeVars.appr (anin : [[G ⊢ a ∉ fvftv(E F)]])
+  : [[G ⊢ a ∉ fvftv(F)]] := by
+  intro ain
+  apply anin
+  let .mk x'infv x'A'inG ainftv := ain
+  exact .mk x'infv.appr x'A'inG ainftv
+
+theorem NotInFreeTermVars'Types'FreeTypeVars.typeGen (anin : [[G ⊢ a ∉ fvftv(Λ b. E)]])
+  : [[G ⊢ a ∉ fvftv(E)]] := by
+  intro ain
+  apply anin
+  let .mk x'infv x'A'inG ainftv := ain
+  exact .mk x'infv.typeGen x'A'inG ainftv
+
+theorem NotInFreeTermVars'Types'FreeTypeVars.typeApp (anin : [[G ⊢ a ∉ fvftv(E [A])]])
+  : [[G ⊢ a ∉ fvftv(E)]] := by
+  intro ain
+  apply anin
+  let .mk x'infv x'A'inG ainftv := ain
+  exact .mk x'infv.typeApp x'A'inG ainftv
+
+judgement_syntax G " ⊢ " E " : " A : Typing
 
 judgement Typing :=
 
 x : A ∈ G
-────────── var
-G |- x : A
+───────── var
+G ⊢ x : A
 
-G |- A
-G, x : A |- E : B
-─────────────────────── lam
-G |- λ x : A. E : A → B
+G ⊢ A
+G, x : A ⊢ E : B
+────────────────────── lam
+G ⊢ λ x : A. E : A → B
 
-G |- E : A → B
-G |- F : A
-────────────── app
-G |- E F : B
+G ⊢ E : A → B
+G ⊢ F : A
+───────────── app
+G ⊢ E F : B
 
-G, a |- E : A
-──────────────────── typeGen
-G |- Λ a. E : ∀ a. A
+G ⊢ a ∉ fvftv(E)
+G, a ⊢ E : A
+─────────────────── typeGen
+G ⊢ Λ a. E : ∀ a. A
 
-G |- E : ∀ a. A
-G |- B
-────────────────────── typeApp
-G |- E [B] : A [a ↦ B]
+G ⊢ E : ∀ a. A
+G ⊢ B
+───────────────────── typeApp
+G ⊢ E [B] : A [a ↦ B]
 
--- TODO: Define operational semantics.
+theorem Typing.TermVar_swap (EtyB : [[G, y : A▁other, x : A, GG ⊢ E : B]]) (xney : x ≠ y)
+  : [[G, x : A, y : A▁other, GG ⊢ E : B]] :=
+  match EtyB with
+  | .var x'BinGyxappGG =>
+    match x'BinGyxappGG.append_elim with
+    | .inl ⟨x'BinGyx, x'ninGG⟩ => match x'BinGyx with
+      | .head => .var <| TermVarInEnvironment.append_inl (.termVarExt .head xney) x'ninGG
+      | .termVarExt x'BinGy x'nex => match x'BinGy with
+        | .head => .var <| .append_inl .head x'ninGG
+        | .termVarExt x'BinG x'ney =>
+          .var <| x'BinG.termVarExt x'nex |>.termVarExt x'ney |>.append_inl x'ninGG
+    | .inr x'BinGG => .var x'BinGG.append_inr
+  | .lam A'wf E'tyB' =>
+    .lam A'wf.TermVar_swap <| E'tyB'.TermVar_swap (GG := GG.termVarExt ..) xney
+  | .app E'tyA'arrB F'tyA' => .app (E'tyA'arrB.TermVar_swap xney) (F'tyA'.TermVar_swap xney)
+  | .typeGen a'nin E'tyA' =>
+    .typeGen (a'nin.TermVar_swap xney) <| E'tyA'.TermVar_swap (GG := GG.typeVarExt _) xney
+  | .typeApp E'ty B'wf => .typeApp (E'ty.TermVar_swap xney) B'wf.TermVar_swap
 
--- TODO: Prove preservation and progress.
+theorem Typing.False_of_in_fv_of_nin_Environment (EtyA : [[G ⊢ E : A]]) (xinfvE : [[x ∈ fv(E)]])
+  (xninG : [[x ∉ G]]) : False :=
+  match EtyA, xinfvE with
+  | .var x'AinG, .var => xninG _ x'AinG
+  | .lam _ E'tyB', .lam xinfvE' xnex' =>
+    E'tyB'.False_of_in_fv_of_nin_Environment xinfvE' (xninG.termVarExt xnex'.symm)
+  | .app E'tyA'arrA F'tyA', .appl xinfvE' =>
+    E'tyA'arrA.False_of_in_fv_of_nin_Environment xinfvE' xninG
+  | .app _ F'tyA', .appr xinfvF' => F'tyA'.False_of_in_fv_of_nin_Environment xinfvF' xninG
+  | .typeGen _ E'tyA', .typeGen xinfvE' =>
+    E'tyA'.False_of_in_fv_of_nin_Environment xinfvE' xninG.typeVarExt
+  | .typeApp E'ty B'wf, .typeApp xinfvE' => E'ty.False_of_in_fv_of_nin_Environment xinfvE' xninG
+
+theorem NotInFreeTermVars'Types'FreeTypeVars.append_inr (anin : [[G ⊢ a ∉ fvftv(E)]])
+  (EtyA : [[G, b ⊢ E : A]]) : [[GG, G ⊢ a ∉ fvftv(E)]] := fun ain =>
+  anin <|
+    let .mk x'infv x'A'inGGappG ainftv := ain
+    match x'A'inGGappG.append_elim with
+    | .inl ⟨_, x'ninG⟩ =>
+      False.elim <| EtyA.False_of_in_fv_of_nin_Environment x'infv x'ninG.typeVarExt
+    | .inr x'A'inG => .mk x'infv x'A'inG ainftv
+
+theorem Typing.append_inr : [[G ⊢ E : A]] → [[GG, G ⊢ E : A]]
+  | .var xAinG => .var xAinG.append_inr
+  | .lam A'wf E'tyB => .lam A'wf.append_inr E'tyB.append_inr
+  | .app FtyA' E'tyA'arrA => .app FtyA'.append_inr E'tyA'arrA.append_inr
+  | .typeGen a'nin E'tyA' => .typeGen (a'nin.append_inr E'tyA') E'tyA'.append_inr
+  | .typeApp E'ty Bwf => .typeApp E'ty.append_inr Bwf.append_inr
+
+theorem Typing.TermVar_shadowed : [[G, x : A▁shadowed, GG, x : A, GGG ⊢ E : B]] → [[G, GG, x : A, GGG ⊢ E : B]]
+  | var x'BinGxGGxGGG =>
+    match x'BinGxGGxGGG.append_elim with
+    | .inl ⟨x'BinGx, x'ninGGxGGG⟩ =>
+      match x'BinGx with
+      | .head => False.elim <| x'ninGGxGGG A <| TermVarInEnvironment.append_inl .head
+          fun A' xA'inGGG => x'ninGGxGGG A' xA'inGGG.append_inr
+      | .termVarExt x'BinG _ => .var <| x'BinG.append_inl x'ninGGxGGG
+    | .inr x'BinGGxGGG => .var x'BinGGxGGG.append_inr
+  | lam A'wf E'tyB' => .lam A'wf.TermVar_drop <| E'tyB'.TermVar_shadowed (GGG := GGG.termVarExt ..)
+  | app E'tyA'arrB FtyA' => .app E'tyA'arrB.TermVar_shadowed FtyA'.TermVar_shadowed
+  | typeGen a'nin E'tyA' => .typeGen a'nin.TermVar_shadowed <| E'tyA'.TermVar_shadowed (GGG := GGG.typeVarExt _)
+  | typeApp E'ty B'wf => .typeApp E'ty.TermVar_shadowed B'wf.TermVar_drop
+
+set_option linter.unusedVariables false in
+theorem Typing.TypeVar_shadowed_subst (EtyA : [[ε, a, G, a, GG ⊢ E : A]]) (Bwf : [[ε ⊢ B]])
+  (aninG : [[a ∉ G]])
+  (ih : ∀ x : TermVar, [[x ∈ fv(E)]] → (∃ A, [[x : A ∈ GG]]) ∨ ∀ A, [[x : A ∈ G]] → [[a ∉ ftv(A)]])
+  : [[(G, a) [a ↦ B], GG ⊢ E : A]] := by
+  cases EtyA
+  · case var x xAinεaGaGG =>
+    match xAinεaGaGG.append_elim with
+    | .inl ⟨xAinεa, _⟩ =>
+      cases xAinεa
+      case typeVarExt xAinε =>
+      cases xAinε
+    | .inr xAinGaGG => match xAinGaGG.append_elim with
+      | .inl ⟨xAinGa, xninGG⟩ =>
+        apply Typing.var
+        apply TermVarInEnvironment.append_inl _ xninGG
+        rw [← Environment.subst_typeVarExt_eq_typeVarExt_subst]
+        apply TermVarInEnvironment.typeVarExt
+        cases xAinGa
+        case a.typeVarExt xAinG =>
+        have aninftvA : [[a ∉ ftv(A)]] := by
+          match ih x .var with
+          | .inl ⟨A', xA'inGG⟩ => exact False.elim <| xninGG A' xA'inGG
+          | .inr h => exact h A xAinG
+        rw [← NotInFreeTypeVars.subst_id aninftvA]
+        exact xAinG.subst aninG
+      | .inr xAinGG => exact .var xAinGG.append_inr
+  · case lam A' x E' B' A'wf E'tyB' =>
+    apply Typing.lam A'wf.TypeVar_shadowed_subst
+    apply E'tyB'.TypeVar_shadowed_subst (GG := GG.termVarExt x A') Bwf aninG
+    intro x' x'infvE'
+    by_cases x' = x
+    · case pos x'eqx =>
+      rw [x'eqx]
+      exact .inl <| Exists.intro A' .head
+    · case neg x'nex =>
+      match ih x' (x'infvE'.lam x'nex) with
+      | .inl ⟨A'', x'A''inGG⟩ => exact .inl <| Exists.intro A'' <| x'A''inGG.termVarExt x'nex
+      | .inr h => exact .inr h
+  · case app E' A' F FtyA' E'tyA'arrA =>
+    exact .app (E'tyA'arrA.TypeVar_shadowed_subst Bwf aninG (ih · ·.appl))
+      (FtyA'.TypeVar_shadowed_subst Bwf aninG (ih · ·.appr))
+  · case typeGen a' E' A' a'nin E'tyA' =>
+    apply Typing.typeGen _ <| E'tyA'.TypeVar_shadowed_subst (GG := GG.typeVarExt a') Bwf aninG _
+    · intro a'in
+      apply a'nin
+      let .mk x'infv x'A'in a'inftv := a'in
+      match x'A'in.append_elim with
+      | .inl ⟨.typeVarExt x'A'in, x'ninGG⟩ =>
+        let ⟨A'', ⟨x'A''in, eq⟩⟩ := x'A'in.unsubst aninG
+        rw [eq] at a'inftv
+        exact .mk x'infv (x'A''in.typeVarExt.append_inl x'ninGG).append_inr <| a'inftv.unsubst Bwf
+      | .inr x'A'inGG => exact .mk x'infv x'A'inGG.append_inr.append_inr a'inftv
+    · intro x xinfvE'
+      match ih x xinfvE'.typeGen with
+      | .inl ⟨A'', x'A''inGG⟩ => exact .inl <| Exists.intro A'' <| x'A''inGG.typeVarExt
+      | .inr h => exact .inr h
+  · case typeApp E' a' A' B' E'ty B'wf =>
+    exact .typeApp (E'ty.TypeVar_shadowed_subst Bwf aninG (ih · ·.typeApp)) B'wf.TypeVar_shadowed_subst
+
+theorem NotInFreeTermVars.of_Typing_of_TermVarNotInEnvironment (EtyA : [[G ⊢ E : A]])
+  (xninG : [[x ∉ G]]) : [[x ∉ fv(E)]] := by
+  intro ain
+  match EtyA, ain with
+  | .var x'inG, .var => exact xninG A x'inG
+  | .lam _ E'tyB, .lam xinE' xnex' =>
+    apply NotInFreeTermVars.of_Typing_of_TermVarNotInEnvironment E'tyB _ xinE'
+    exact xninG.termVarExt xnex'.symm
+  | .app E'tyA'arrA _, .appl xinE' =>
+    exact NotInFreeTermVars.of_Typing_of_TermVarNotInEnvironment E'tyA'arrA xninG xinE'
+  | .app _ F'tyA', .appr xinF' =>
+    exact NotInFreeTermVars.of_Typing_of_TermVarNotInEnvironment F'tyA' xninG xinF'
+  | .typeGen _ E'tyA', .typeGen xinE' =>
+    exact NotInFreeTermVars.of_Typing_of_TermVarNotInEnvironment E'tyA' xninG.typeVarExt xinE'
+  | .typeApp E'ty _, .typeApp xinE' =>
+    exact NotInFreeTermVars.of_Typing_of_TermVarNotInEnvironment E'ty xninG xinE'
+
+theorem InFreeTermVars.untmSubst (xin : [[x ∈ fv(E [y ↦ F])]]) (FtyA : [[ε ⊢ F : A]])
+  : [[x ∈ fv(E)]] := by
+  match E with
+  | .var x' =>
+    rw [Term.tmSubst] at xin
+    split at xin
+    · case isTrue x'eqx =>
+      exact False.elim <|
+        NotInFreeTermVars.of_Typing_of_TermVarNotInEnvironment FtyA TermVarNotInEnvironment.ε xin
+    · case isFalse x'nex =>
+      let .var := xin
+      exact .var
+  | .lam x' A' E' =>
+    rw [Term.tmSubst] at xin
+    split at xin
+    · case isTrue x'eqy => exact xin
+    · case isFalse x'ney =>
+      let .lam xinE' xnex' := xin
+      exact .lam (xinE'.untmSubst FtyA) xnex'
+  | .app E' F' =>
+    rw [Term.tmSubst] at xin
+    match xin with
+    | .appl xinE' => exact .appl <| xinE'.untmSubst FtyA
+    | .appr xinF' => exact .appr <| xinF'.untmSubst FtyA
+  | .typeGen a' E' =>
+    rw [Term.tmSubst] at xin
+    let .typeGen xinE' := xin
+    exact .typeGen <| xinE'.untmSubst FtyA
+  | .typeApp E' A'' =>
+    rw [Term.tmSubst] at xin
+    let .typeApp xinE' := xin
+    exact .typeApp <| xinE'.untmSubst FtyA
+
+theorem NotInFreeTermVars'Types'FreeTypeVars.Term_tmSubst (anin : [[G ⊢ a ∉ fvftv(E)]])
+  (FtyA : [[ε ⊢ F : A]]) : [[G ⊢ a ∉ fvftv(E [x ↦ F])]] := by
+  intro ain
+  apply anin
+  cases ain
+  case mk x' A' x'A'inG ainftv x'infv =>
+  exact InFreeTermVars'Types'FreeTypeVars.mk (x'infv.untmSubst FtyA) x'A'inG ainftv
+
+theorem InFreeTermVars.untySubst (xin : [[x ∈ fv(E [b ↦ B])]]) : [[x ∈ fv(E)]] := by
+  match E with
+  | .var x' =>
+    rw [Term.tySubst] at xin
+    exact xin
+  | .lam x' A' E' =>
+    rw [Term.tySubst] at xin
+    let .lam xinE' xnex' := xin
+    exact InFreeTermVars.lam xinE'.untySubst xnex'
+  | .app E' F' =>
+    rw [Term.tySubst] at xin
+    match xin with
+    | .appl xinE' => exact .appl xinE'.untySubst
+    | .appr xinF' => exact .appr xinF'.untySubst
+  | .typeGen a' E' =>
+    rw [Term.tySubst] at xin
+    split at xin
+    · case isTrue a'eqb => exact xin
+    · case isFalse a'neb =>
+      let .typeGen xinE' := xin
+      exact .typeGen xinE'.untySubst
+  | .typeApp E' A'' =>
+    rw [Term.tySubst] at xin
+    let .typeApp xinE' := xin
+    exact .typeApp xinE'.untySubst
+
+theorem NotInFreeTermVars'Types'FreeTypeVars.Term_tySubst (anin : [[G ⊢ a ∉ fvftv(E)]])
+  : [[G ⊢ a ∉ fvftv(E [b ↦ A])]] := by
+  intro ain
+  apply anin
+  cases ain
+  case mk x' A' x'A'inG ainftv x'infv =>
+  exact InFreeTermVars'Types'FreeTypeVars.mk x'infv.untySubst x'A'inG ainftv
+
+theorem Typing.tmSubst_preservation (EtyB : [[ε, x : A, G ⊢ E : B]]) (xninG : [[x ∉ G]])
+  (FtyA : [[ε ⊢ F : A]]) : [[G ⊢ E [x ↦ F] : B]] := by
+  match EtyB with
+  | .var x'BinεxappG =>
+    rw [Term.tmSubst]
+    split
+    · case isTrue x'eqx =>
+      rw [x'eqx] at x'BinεxappG
+      match x'BinεxappG.append_elim with
+      | .inl ⟨xBinεx, _⟩ =>
+        cases xBinεx
+        · case head => exact FtyA.append_inr
+        · case termVarExt xBinε xnex => contradiction
+      | .inr xBinG =>
+        exact False.elim <| xninG B xBinG
+    · case isFalse x'nex =>
+      match x'BinεxappG.append_elim with
+      | .inl ⟨xBinGx, xninG⟩ =>
+        cases xBinGx
+        · case head => contradiction
+        · case termVarExt x'Binε _ => cases x'Binε
+      | .inr x'BinG => exact .var x'BinG
+  | .lam A'wf E'tyB' =>
+    rw [Term.tmSubst]
+    split
+    · case isTrue x'eqx =>
+      rw [x'eqx, G.empty_append]
+      rw [x'eqx] at E'tyB'
+      exact .lam A'wf.TermVar_drop <| E'tyB'.TermVar_shadowed (GGG := .empty)
+    · case isFalse x'nex =>
+      rw [G.empty_append]
+      apply Typing.lam A'wf.TermVar_drop
+      rw [← G.empty_append]
+      apply E'tyB'.tmSubst_preservation (G := G.termVarExt ..) _ FtyA
+      exact xninG.termVarExt x'nex
+  | .app E'tyA'arrB F'tyA' =>
+    exact .app (E'tyA'arrB.tmSubst_preservation xninG FtyA) (F'tyA'.tmSubst_preservation xninG FtyA)
+  | .typeGen a'nin E'tyA' =>
+    apply Typing.typeGen <| a'nin.append_elr.Term_tmSubst FtyA
+    apply E'tyA'.tmSubst_preservation (G := G.typeVarExt _) _ FtyA
+    exact xninG.typeVarExt
+  | .typeApp E'ty B'wf =>
+    apply Typing.typeApp <| E'ty.tmSubst_preservation xninG FtyA
+    rw [G.empty_append]
+    exact B'wf.TermVar_drop
+
+theorem Typing.tySubst_preservation (EtyA : [[ε, a, G ⊢ E : A]]) (aninG : [[a ∉ G]])
+  (Bwf : [[ε ⊢ B]]) : [[G [a ↦ B] ⊢ E [a ↦ B] : A [a ↦ B] ]] := by
+  cases EtyA
+  · case var x xAinεaappG => match xAinεaappG.append_elim with
+    | .inr xAinG => exact .var <| xAinG.subst aninG
+  · case lam A' x E' B' A'wf E'tyB' =>
+    rw [Term.tySubst]
+    rw [← Environment.append] at E'tyB'
+    apply Typing.lam (A'wf.subst Bwf)
+    rw [Environment.subst_termVarExt_eq_termVarExt_subst_of_TypeVarNotInEnvironment aninG]
+    exact E'tyB'.tySubst_preservation (G := G.termVarExt x A') aninG.termVarExt Bwf
+  · case app E' A' F FtyA' E'tyA'arrA =>
+    exact .app (E'tyA'arrA.tySubst_preservation aninG Bwf) (FtyA'.tySubst_preservation aninG Bwf)
+  · case typeGen a' E' A' a'nin E'tyA' =>
+    rw [Term.tySubst]
+    split
+    · case isTrue a'eqa =>
+      rw [a'eqa]
+      rw [a'eqa] at E'tyA' a'nin
+      apply Typing.typeGen <| a'nin.append_elr.Environment_subst Bwf aninG
+      rw [if_pos rfl, Environment.subst_typeVarExt_eq_typeVarExt_subst]
+      apply E'tyA'.TypeVar_shadowed_subst (GG := .empty) Bwf aninG
+      intro x xinfvE'
+      right
+      intro A'' xA''inG ainftvA''
+      exact a'nin <| InFreeTermVars'Types'FreeTypeVars.mk xinfvE' xA''inG.append_inr ainftvA''
+    · case isFalse a'nea =>
+      apply Typing.typeGen <| a'nin.append_elr.Term_tySubst.Environment_subst Bwf aninG
+      rw [if_neg a'nea, Environment.subst_typeVarExt_eq_typeVarExt_subst]
+      exact E'tyA'.tySubst_preservation (G := G.typeVarExt a') (aninG.typeVarExt a'nea) Bwf
+  · case typeApp E' a' A' B' E'ty B'wf =>
+    rw [Term.tySubst]
+    by_cases a' = a
+    · case pos a'eqa =>
+      rw [a'eqa, Type'.subst_subst]
+      rw [a'eqa] at E'ty
+      apply Typing.typeApp _ (B'wf.subst Bwf)
+      rw [Type'.subst_shadowed_forall B]
+      exact E'ty.tySubst_preservation aninG Bwf
+    · case neg a'nea =>
+      -- TODO: Probably need to use alpha equivalence to avoid issues when B' contains a.
+      have : ((A'.subst a' B').subst a B) = (A'.subst a B).subst a' (B'.subst a B) := sorry
+      rw [this]
+      apply Typing.typeApp _ <| B'wf.subst Bwf
+      rw [Type'.forall_subst_eq_subst_forall a'nea]
+      exact E'ty.tySubst_preservation aninG Bwf
+
+judgement_syntax "⊢ " E " -> " F : OperationalSemantics
+
+judgement OperationalSemantics :=
+
+⊢ E -> E▁next
+───────────────── appl
+⊢ E F -> E▁next F
+
+⊢ F -> F▁next
+───────────────── appr
+⊢ V F -> V F▁next
+
+───────────────────────────── lamApp
+⊢ (λ x : A. E) V -> E [x ↦ V]
+
+⊢ E -> E▁next
+───────────────────── typeApp
+⊢ E [A] -> E▁next [A]
+
+─────────────────────────── typeGenApp
+⊢ (Λ a. E) [A] -> E [a ↦ A]
+
+theorem preservation (EtyA : [[ε ⊢ E : A]]) (EstepF : [[⊢ E -> F]]) : [[ε ⊢ F : A]] :=
+  match EstepF, EtyA with
+  | .appl E'stepE'next, .app E'tyA'arrA FtyA' => .app (preservation E'tyA'arrA E'stepE'next) FtyA'
+  | .appr FstepFnext, .app VtyA'arrA FtyA' => .app VtyA'arrA <| preservation FtyA' FstepFnext
+  | .lamApp, .app (.lam _ E'tyA) VtyA'' =>
+      E'tyA.tmSubst_preservation (G := .empty) TermVarNotInEnvironment.ε VtyA''
+  | .typeApp E'stepE'next, .typeApp E'ty A'wf => .typeApp (preservation E'ty E'stepE'next) A'wf
+  | .typeGenApp, .typeApp (.typeGen _ E'tyA'') A'wf =>
+    E'tyA''.tySubst_preservation (G := .empty) TypeVarNotInEnvironment.ε A'wf
+
+set_option linter.unusedVariables false in
+theorem progress (EtyA : [[ε ⊢ E : A]]) : (∃ F, [[⊢ E -> F]]) ∨ ∃ V : Value, V.val = E :=
+  match E, EtyA with
+  | .lam x A' E', _ => .inr <| Exists.intro { val := .lam x A' E', property := by simp } rfl
+  | .app E' F', .app E'tyA'arrA F'tyA' =>
+    match progress E'tyA'arrA with
+    | .inl ⟨E'_next, E'stepE'_next⟩ => .inl <| Exists.intro (E'_next.app F') (.appl E'stepE'_next)
+    | .inr ⟨VE', VE'eqE'⟩ => by
+      match progress F'tyA' with
+      | .inl ⟨F'_next, F'stepF'_next⟩ =>
+        rw [← VE'eqE']
+        exact .inl <| Exists.intro (VE'.val.app F'_next) (.appr F'stepF'_next)
+      | .inr ⟨VF', VF'eqF'⟩ =>
+        have E'val := VE'.property
+        rw [VE'eqE'] at E'val
+        match E' with
+        | .lam x A' E'' =>
+          rw [← VF'eqF']
+          exact .inl <| Exists.intro (E''.tmSubst x VF'.val) .lamApp
+  | .typeGen a E', _ => .inr <| Exists.intro { val := .typeGen a E', property := by simp } rfl
+  | .typeApp E' A', .typeApp E'ty A'wf =>
+    match progress E'ty with
+    | .inl ⟨E'_next, E'stepE'_next⟩ =>
+      .inl <| Exists.intro (E'_next.typeApp A') <| .typeApp E'stepE'_next
+    | .inr ⟨VE', VE'eqE'⟩ => by
+      have E'val := VE'.property
+      rw [VE'eqE'] at E'val
+      match E' with
+      | .typeGen a E'' => exact .inl <| Exists.intro (E''.tySubst a A') .typeGenApp
 
 end LottExamples.SystemF
